wrote a general lemma about om_trans PF change

fairness/lawyer/obligations/obls_termination.v
@@ -4,7 +4,7 @@ From trillium.fairness Require Import locales_helpers inftraces fairness trace_l
 From trillium.fairness.lawyer.obligations Require Import obligations_model multiset_utils obls_utils.
 From stdpp Require Import relations.
 Require Import Coq.Program.Wf.
-
+Require Import Relation_Operators.
 
 Definition maximal {A C : Type} {H : ElemOf A C} (R : relation A) (x : A) (X : C) :=
   minimal (flip R) x X.
@@ -54,7 +54,7 @@ Section Termination.
 
     Definition approx_expects (k: nat) (eps: gset (@ExpectPermission Degree)) :=
       ([^op set] ep ∈ eps, let '(sid, π, d) := ep in
-        (2 * (LIM_STEPS + 2) * set_before sid - k) *: {[+ d +]}
+        ((LIM_STEPS + 2) * set_before sid - k) *: {[+ d +]}
       ).
 
     Instance cmp_phase'_dec: forall (x y: Phase * Degree),
@@ -96,9 +96,18 @@ Section Termination.
       apply scalar_mul_le. lia.
     Qed.
 
+    Lemma ms_le_PF_le m n π δ
+      (LE: m <= n):
+      ms_le deg_le (PF π n δ) (PF π m δ).
+    Proof using.
+      apply ms_le_disj_union.
+      + apply ms_le_sub. apply mset_map_sub. apply mset_filter_subseteq_mono. mss.
+      + apply ms_le_exp_le. lia.
+    Qed. 
+
     Lemma approx_expects_add k eps e 
       (FRESH: e ∉ eps):
-      let n := (2 * (LIM_STEPS + 2) * set_before (fst $ fst e) - k) in
+      let n := ((LIM_STEPS + 2) * set_before (fst $ fst e) - k) in
       approx_expects k (eps ∪ {[ e ]}) = approx_expects k eps ⊎ n *: {[+ e.2 +]}.
     Proof using.
       rewrite (union_comm_L _ {[ e ]}).
@@ -213,20 +222,34 @@ Section Termination.
           * eapply elem_of_mset_map. eexists (_, _). split; eauto.
             apply mset_filter_spec. split; eauto. 
           * done. 
-    Qed. 
+    Qed.
 
-    Lemma other_loc_step_ms_le π__ow δ1 τ δ2 k
-      (STEP: loc_step OP δ1 τ δ2)
-      (OTHER:
-        let π := default π0 (ps_phases _ δ1 !! τ) in
-        phases_incompat π__ow π):
-      ms_le deg_le (PF π__ow (S k) δ2) (PF π__ow k δ1).
+    Definition expect_ms_le π δ1 τ δ2 k :=
+      forall sid π' d,
+        expects_ep _ δ1 τ δ2 sid π' d ->
+        ms_le deg_le (PF π (S k) δ2) (PF π k δ1). 
+
+    Lemma loc_step_ms_le π δ1 τ δ2 k
+      (STEP: loc_step _ δ1 τ δ2)
+      (EXP_CASE: expect_ms_le π δ1 τ δ2 k)
+      :
+      ms_le deg_le (PF π (S k) δ2) (PF π k δ1).
     Proof using.
       clear LVL_WF.
-      rewrite /PF.
       apply loc_step_split in STEP as [NOEXP | EXP].
-      { eapply loc_step_no_exp_all_ms_le; eauto. }
-      destruct EXP as (?&?&?&T). inversion T; subst.
+      - eapply loc_step_no_exp_all_ms_le; eauto.
+      - destruct EXP as (?&?&?&?). eapply EXP_CASE; eauto.
+    Qed. 
+
+    Lemma other_expect_ms_le π__ow δ1 τ δ2 k
+      (OTHER: let π := default π0 (ps_phases _ δ1 !! τ) in
+              phases_incompat π__ow π):
+      expect_ms_le π__ow δ1 τ δ2 k. 
+    Proof using.
+      clear LVL_WF. 
+      red. intros sid π' d EXP. 
+      rewrite /PF.
+      inversion EXP; subst.
       destruct δ1. simpl in *.
       subst new_cps0.
       
@@ -241,23 +264,21 @@ Section Termination.
       + apply ms_le_exp_le. lia. 
     Qed.
 
-    Lemma min_owner_loc_step_ms_le δ1 τ δ2 k (* s l *)
-      (STEP: loc_step OP δ1 τ δ2)
+    Lemma min_owner_expect_ms_le δ1 τ δ2 k
       (SET_BOUND: forall sid π d, expects_ep OP δ1 τ δ2 sid π d ->
-                  let n := 2 * (LIM_STEPS + 2) * set_before sid in
+                  let n := (LIM_STEPS + 2) * set_before sid in
                   k < n)
       :
       let π__ow := default π0 (ps_phases _ δ1 !! τ) in
-      ms_le deg_le (PF π__ow (S k) δ2) (PF π__ow k δ1).
+      expect_ms_le π__ow δ1 τ δ2 k. 
     Proof using.
       clear LVL_WF. 
+      intros. red. intros sid π' d EXP. 
       rewrite /PF.
-      apply loc_step_split in STEP as [NOEXP | EXP].
-      { eapply loc_step_no_exp_all_ms_le; eauto. }
 
-      destruct EXP as (?&?&?&T). inversion T; subst.
-      destruct δ1. simpl in *.
-      subst new_cps0. rewrite LOC_PHASE. simpl. 
+      inversion EXP; subst.
+      destruct δ1. simpl in *. subst new_cps0.
+      subst π__ow. rewrite LOC_PHASE. simpl. 
       
       rewrite !mset_filter_disj_union mset_map_disj_union.
       rewrite !mset_filter_singleton.
@@ -285,22 +306,181 @@ Section Termination.
       rewrite -gmultiset_scalar_mul_S_r. f_equiv. lia.
     Qed.
 
+    Definition nsteps_keep_ms_le π δ i τ :=
+      forall δ' k
+      (ITH: tr S!! i = Some δ)
+      (BOUND : k ≤ LIM_STEPS)
+      (STEPS: nsteps (λ p1 p2, loc_step OP p1 τ p2) k δ δ'),
+      ms_le deg_le (PF π ((LIM_STEPS + 2) * i + k) δ') (PF π ((LIM_STEPS + 2) * i) δ).
+
+    Lemma forks_locale_ms_le π δ1 τ δ2 τ' R k
+      (FORK: forks_locale OP δ1 τ δ2 τ' R):
+      ms_le deg_le (PF π (S k) δ2) (PF π k δ1).
+    Proof using.
+      rewrite /PF.
+      inversion FORK; subst. 
+      destruct δ1. simpl in *.
+      apply ms_le_disj_union.
+      + apply ms_le_sub. apply mset_map_sub. mss. 
+      + apply ms_le_exp_le. lia.
+    Qed.
+
+    Lemma om_trans_ms_rel (bd: bool) π i
+      (rel := (if bd then ms_lt deg_le else ms_le deg_le): relation (gmultiset Degree))
+      (VALID: obls_trace_valid OP tr)
+      (BURN_REL:
+        forall δ δ' τ mb mf k,
+          tr !! i = Some (δ, Some (τ, δ')) ->
+          k ≤ LIM_STEPS ->
+          nsteps (λ p1 p2, loc_step OP p1 τ p2) k δ mb ->
+          (∃ π δ, burns_cp OP mb τ mf π δ) ->
+          clos_refl (ProgressState OP) (λ p1 p2, ∃ τ' R, forks_locale OP p1 τ p2 τ' R) mf δ' ->
+          rel (PF π ((LIM_STEPS + 2) * i + LIM_STEPS + 1) mf) (PF π ((LIM_STEPS + 2) * i + LIM_STEPS) mb))
+      (NSTEPS_LE: forall δ τ i,
+          tr S!! i = Some δ ->
+          tr L!! i = Some τ ->
+          nsteps_keep_ms_le π δ i τ)
+      (DOM: is_Some (tr S!! (S i))):
+      rel (TPF π (S i)) (TPF π i).
+    Proof using.
+      rewrite /TPF. simpl.
+      forward eapply (proj2 (label_lookup_states' _ _)) as [τ ITHl]; eauto.  
+      forward eapply (state_lookup_prev _ _ DOM _ (PeanoNat.Nat.le_succ_diag_r _)).
+      intros [δ ITH]. destruct DOM as [δ' ITH']. rewrite ITH ITH'. simpl. 
+
+      forward eapply trace_valid_steps'' as STEP; eauto.
+      { rewrite Nat.add_1_r. eauto. }
+      simpl in STEP. red in STEP. destruct STEP as (mf & PSTEP & FSTEP).
+      red in PSTEP. destruct PSTEP as (k & BOUND & (mb & PSTEP & BSTEP)).
+
+      eapply BURN_REL in BSTEP; eauto.
+      2: { eapply state_label_lookup; eauto. rewrite Nat.add_1_r. eauto. }
+      eapply NSTEPS_LE in PSTEP; eauto. 
+
+      assert (ms_le deg_le (PF π ((LIM_STEPS + 2) * S i) δ')
+            (PF π ((LIM_STEPS + 2) * i + LIM_STEPS + 1) mf)).
+      { inversion FSTEP.
+        2: { subst mf.
+             rewrite /PF. apply ms_le_disj_union.
+             - reflexivity.
+             - apply ms_le_exp_le. lia. }
+        destruct H0 as (?&?&?). 
+        subst y. eapply ms_le_Proper; [| reflexivity| eapply forks_locale_ms_le; eauto].
+        f_equiv. apply leibniz_equiv_iff. lia. }  
+
+      destruct bd; subst rel.
+      - eapply strict_transitive_l; [| apply PSTEP]. 
+        eapply strict_transitive_r; [apply H0| ]. 
+        eapply strict_transitive_l; [apply BSTEP| ].
+        apply ms_le_PF_le. lia.
+      - etrans; [| apply PSTEP].
+        etrans; [apply H0| ].
+        etrans; [apply BSTEP| ].
+        apply ms_le_PF_le. lia.
+    Qed.        
+
+
+    foobar. 
+    Lemma tr_loc_step_nsteps_ms_le π δ i τ δ' k
+      (ITH: tr S!! i = Some δ)
+      (BOUND : k ≤ LIM_STEPS)
+      (STEPS: nsteps (λ p1 p2, loc_step OP p1 τ p2) k δ δ'):
+      ms_le deg_le (PF π (2 * (LIM_STEPS + 2) * i + k) δ') (PF π (2 * (LIM_STEPS + 2) * i) δ).
+    Proof using.
+      generalize dependent δ'.
+      induction k.
+      { intros ? ->%obls_utils.nsteps_0.
+        rewrite Nat.add_0_r. reflexivity. }
+      intros δ'' (δ' & STEPS & STEP)%nsteps_inv_r.
+      specialize (IHk ltac:(lia) _ STEPS).
+      etrans; eauto.
+
+      eapply ms_le_Proper; [| | eapply loc_step_ms_le]; eauto.
+      { rewrite -PeanoNat.Nat.add_succ_comm. simpl. reflexivity. }
+      red. 
+
+      eapply loc_step_ms_le. 
+
+      (* follows from well-formedness of state *)
+      assert (ps_phases OP δ !! τ = Some π__ow) as PH by admit. rewrite PH. simpl. 
+      (* follows from preservation of phases before fork *)
+      assert (ps_phases OP δ' !! τ = Some π__ow) as PH' by admit. 
+      
+      eapply ms_le_Proper; [| | eapply min_owner_loc_step_ms_le]; eauto.
+      { rewrite PH'.
+        rewrite -PeanoNat.Nat.add_succ_comm. simpl. reflexivity. }
+      { rewrite PH'. simpl. reflexivity. }
+
+      intros sid π d EXP. simpl.
+      inversion EXP. subst.
+      rewrite PH' in LOC_PHASE. inversion LOC_PHASE. subst π__max.
+
+      enough (set_before sid > i).
+      { apply PeanoNat.Nat.le_succ_l in H0. 
+        apply Nat.le_sum in H0 as [u EQ]. rewrite EQ. lia. }
+
+      clear -NEVER_SET ITH OBLS_LT SET_BEFORE_SPEC MIN.
+
+      foobar.
+
+
+
     Hypothesis (SET_BEFORE_SPEC: 
                  forall sid i,
                    (forall c, ¬ never_set_after sid c) ->
                    set_before sid <= i ->
                    from_option (fun δ => from_option snd false (ps_sigs _ δ !! sid)) false (tr S!! i) = true).
 
-    Lemma tr_loc_step_nsteps_ms_le δ i τ δ' s k
+    Lemma other_sig_exp_lim (δ : ObligationsModel OP) (i : nat) (τ : Locale)
+      (s : SignalId) (δ' : ProgressState OP) (sid : SignalId) (l : Level)
+      (ITH : tr S!! i = Some δ)
+      (NEVER_SET : never_set_after s i)
+      (MIN: minimal_in_prop tr_sig_lt (s, i) (λ sn, never_set_after sn.1 sn.2))
+      (OWNER: s ∈ default ∅ (ps_obls _ δ !! τ))
+      (OBLS_LT : lt_locale_obls OP l τ δ'):
+      i < set_before sid.
+    Proof using. 
+      red in OBLS_LT. red in OBLS_LT.
+      
+      move NEVER_SET at bottom. red in NEVER_SET.
+      specialize (NEVER_SET _ ltac:(reflexivity)).
+      rewrite ITH in NEVER_SET. simpl in NEVER_SET. 
+      destruct (ps_sigs OP δ !! s) as [[ls ?]|] eqn:SIG__min; [| done].
+      simpl in NEVER_SET. subst. 
+      
+      assert (ps_sigs _ δ' !! s = Some (ls, false)) as SIG' by admit.
+      assert (s ∈ default ∅ (ps_obls _ δ' !! τ)) as OBL' by admit.
+      specialize (OBLS_LT ls). specialize_full OBLS_LT.
+      { apply extract_Somes_gset_spec.
+        destruct (ps_obls OP δ' !! τ) as [obs| ] eqn:OBLS'; [| set_solver].
+        simpl in OBL'. simpl. apply elem_of_map. eexists. split; eauto.
+        rewrite SIG'. done. }      
+      
+      red. destruct (Nat.lt_ge_cases i (set_before sid)) as [?|GE]; [done| ].   
+
+      (* either it was there when the big step started,
+         or it's a new signal, but then the thread holds an obligation
+         and cannot wait on it *)
+      assert (ps_sigs OP δ !! sid = Some (l, false)) as SIG0 by admit.
+
+      pose proof (SET_BEFORE_SPEC sid i). specialize_full H0; [| done| ].
+      2: { rewrite ITH in H0. simpl in H0.
+           rewrite SIG0 in H0. done. }
+
+      intros c NEVER_SET_.
+      assert (never_set_after sid i) as NEVER_SET' by admit. clear NEVER_SET_.
+      move MIN at bottom. red in MIN. specialize (MIN (_, _) NEVER_SET').
+      rewrite /tr_sig_lt /MR in MIN. simpl in MIN.
+      rewrite ITH in MIN. simpl in MIN. rewrite SIG0 SIG__min in MIN. simpl in MIN.
+      specialize (MIN OBLS_LT).
+      edestruct @strict_not_both; eauto. 
+    Admitted.
+      
+
+    (* TODO: remove this copy? *)
+    Lemma tr_loc_step_nsteps_ms_le δ i τ δ' k
       (ITH: tr S!! i = Some δ)
       (BOUND : k ≤ LIM_STEPS)
-
-      (NEVER_SET : never_set_after s i)
-      (MIN: minimal_in_prop tr_sig_lt (s, i)
-          (λ ab : SignalId * nat, never_set_after ab.1 ab.2))
-
-      (OWNER: s ∈ default ∅ (ps_obls _ δ !! τ))
-
       (STEPS: nsteps (λ p1 p2, loc_step OP p1 τ p2) k δ δ'):
       let π__ow := default π0 (ps_phases _ δ !! τ) in
       ms_le deg_le (PF π__ow (2 * (LIM_STEPS + 2) * i + k) δ') (PF π__ow (2 * (LIM_STEPS + 2) * i) δ).
@@ -326,44 +506,14 @@ Section Termination.
       intros sid π d EXP. simpl.
       inversion EXP. subst.
       rewrite PH' in LOC_PHASE. inversion LOC_PHASE. subst π__max.
-      red in OBLS_LT. red in OBLS_LT.
-
-      move NEVER_SET at bottom. red in NEVER_SET.
-      specialize (NEVER_SET _ ltac:(reflexivity)).
-      rewrite ITH in NEVER_SET. simpl in NEVER_SET. 
-      destruct (ps_sigs OP δ !! s) as [[ls ?]|] eqn:SIG__min; [| done].
-      simpl in NEVER_SET. subst. 
-      
-      assert (ps_sigs _ δ' !! s = Some (ls, false)) as SIG' by admit.
-      assert (s ∈ default ∅ (ps_obls _ δ' !! τ)) as OBL' by admit.
-      specialize (OBLS_LT ls). specialize_full OBLS_LT.
-      { apply extract_Somes_gset_spec.
-        destruct (ps_obls OP δ' !! τ) as [obs| ] eqn:OBLS'; [| set_solver].
-        simpl in OBL'. simpl. apply elem_of_map. eexists. split; eauto.
-        rewrite SIG'. done. }
 
       enough (set_before sid > i).
       { apply PeanoNat.Nat.le_succ_l in H0. 
         apply Nat.le_sum in H0 as [u EQ]. rewrite EQ. lia. }
-      red. destruct (Nat.lt_ge_cases i (set_before sid)) as [?|GE]; [done| ].   
 
-      (* either it was there when the big step started,
-         or it's a new signal, but then the thread holds an obligation
-         and cannot wait on it *)
-      assert (ps_sigs OP δ !! sid = Some (l, false)) as SIG0 by admit.
+      clear -NEVER_SET ITH OBLS_LT SET_BEFORE_SPEC MIN.
 
-      pose proof (SET_BEFORE_SPEC sid i). specialize_full H0; [| done| ].
-      2: { rewrite ITH in H0. simpl in H0.
-           rewrite SIG0 in H0. done. }
 
-      intros c NEVER_SET_.
-      assert (never_set_after sid i) as NEVER_SET' by admit. clear NEVER_SET_.
-      move MIN at bottom. red in MIN. specialize (MIN (_, _) NEVER_SET').
-      rewrite /tr_sig_lt /MR in MIN. simpl in MIN.
-      rewrite ITH in MIN. simpl in MIN. rewrite SIG0 SIG__min in MIN. simpl in MIN.
-      specialize (MIN OBLS_LT).
-      edestruct @strict_not_both; eauto. 
-    Admitted.
 
     Theorem signals_eventually_set:
       ¬ exists sid c, never_set_after sid c. 
